Ida e volta do lemma de IE (um passo) concluidas. Lemmas auxiliares pendentes.

Lambda_Int_Ext.v
@@ -6,33 +6,6 @@ Require Import Equation_C Lambda Lambda_Ex.
 
 
 
-(*Inductive lab_x_e: pterm -> pterm -> Prop :=*)
-(*| xe_left_app : forall t1 t2 t1', *)
-        (*lab_term(pterm_app t1 t2) ->*)
-        (*t1 ->_Bx t1' ->*)
-        (*lab_x_e (pterm_app t1 t2) (pterm_app t1' t2) *)
-(*| xe_right_app : forall t1 t2 t2', *)
-        (*lab_term(pterm_app t1 t2) ->*)
-        (*t2 ->_Bx t2' ->*)
-        (*lab_x_e (pterm_app t1 t2) (pterm_app t1 t2') *)
-(*| xe_in_lamb : forall t1 t1' L, *)
-        (*lab_term (pterm_abs t1) -> *)
-        (*(forall x, x \notin L ->  (t1 ^ x) ->_Bx (t1' ^ x)) -> *)
-        (*lab_x_e (pterm_abs t1) (pterm_abs t1') *)
-(*| xe_in_es_ext : forall t t' u,*)
-        (*lab_term (t [u]) ->*)
-        (*t ->_Bx t' ->*)
-        (*lab_x_e (t [u]) (t' [u])*)
-(*| xe_in_es_int : forall t t' u,*)
-        (*lab_term (u [t]) ->*)
-        (*t ->_Bx t' ->*)
-        (*lab_x_e (u [t]) (u [t'])*)
-(*| xe_in_les : forall t t' u,*)
-        (*lab_term (t [[u]]) ->*)
-        (*t ->_Bx t' ->*)
-        (*lab_x_e (t [[u]]) (t' [[u]])*)
-(*.*)
-
 Inductive ext_lab_contextual_closure (Red : pterm -> pterm -> Prop) : pterm -> pterm -> Prop :=
 | lab_redex : forall t s, Red t s -> ext_lab_contextual_closure Red t s
 | lab_app_left : forall t t' u, lab_term u -> ext_lab_contextual_closure Red t t' -> 
@@ -62,12 +35,15 @@ Inductive lab_x_i: pterm -> pterm -> Prop :=
                 lab_x_i t t'. 
 
 Definition lab_EE_ctx_red (R: pterm -> pterm -> Prop) (t: pterm) (u : pterm) := 
+    exists t' u', (t =EE t')/\(lab_contextual_closure R t' u')/\(u' =EE u).
+
+Definition ext_lab_EE_ctx_red (R: pterm -> pterm -> Prop) (t: pterm) (u : pterm) := 
     exists t' u', (t =EE t')/\(ext_lab_contextual_closure R t' u')/\(u' =EE u).
 
 
-Definition lab_x_i_eq := lab_EE_ctx_red lab_x_i.
+Definition lab_x_i_eq := ext_lab_EE_ctx_red lab_x_i.
 
-Definition lab_x_e_eq := lab_EE_ctx_red sys_Bx.
+Definition lab_x_e_eq := ext_lab_EE_ctx_red sys_Bx.
 
 Notation "t -->[lx_i] u" := (lab_x_i_eq t u) (at level 59, left associativity).
 Notation "t -->[lx_e] u" := (lab_x_e_eq t u) (at level 59, left associativity).
@@ -122,9 +98,11 @@ Lemma star_ctx_eqcc_lab_term: forall t t', lab_term t -> t =EE t' -> lab_term t'
 Proof.
     Admitted.
 
-Lemma pterm_app_EE_inversion: forall t u v, (pterm_app t u) =EE v -> exists t' u', v = (pterm_app t' u') /\ (t =EE t') /\ (u =EE u').
-Proof.
-    Admitted.
+(*Lemma pterm_app_EE_inversion: forall t u v, (pterm_app t u) =EE v -> exists t' u', v = (pterm_app t' u') /\ (t =EE t') /\ (u =EE u').*)
+(*Proof.*)
+    (*Admitted.*)
+
+(* ------------- star_lab clos *)
 
 Lemma star_lab_closure_app_left: forall R t t' u, lab_term u -> star_closure (lab_contextual_closure R) t t' -> star_closure (lab_contextual_closure R) (pterm_app t u) (pterm_app t' u).
 Proof.
@@ -147,6 +125,8 @@ Proof.
     constructor. constructor 3; auto.
     constructor 2 with (pterm_app u u0); auto.
 Qed.
+
+(* -------------------  EE clos *)
 
 Lemma EE_clos_app_left: forall R t t' u, lab_term u -> ((lab_EE_ctx_red R) t t') -> ((lab_EE_ctx_red R) (pterm_app t u) (pterm_app t' u)).
 Proof.
@@ -196,9 +176,62 @@ Lemma EE_clos_inner_lsub: forall R t u u', (lab_EE_ctx_red R) (u) (u') -> (lab_E
 Proof.
     Admitted.
 
-Lemma pterm_abs_EE_inversion: forall t v, (pterm_abs t) =EE v -> exists t', v = (pterm_abs t') /\ (t =EE t').
+(* -------------------  EE ext_clos *)
+
+Lemma EE_ext_clos_app_left: forall R t t' u, lab_term u -> ((ext_lab_EE_ctx_red R) t t') -> ((ext_lab_EE_ctx_red R) (pterm_app t u) (pterm_app t' u)).
+Proof.
+    intros.
+    destruct H0.
+    destruct H0.
+    destruct H0.
+    destruct H1.
+    exists (pterm_app x u) (pterm_app x0 u).
+    split. apply star_lab_closure_app_left; auto.
+    split*. constructor 2; auto.
+    apply star_lab_closure_app_left; auto.
+
+Qed.
+
+Lemma EE_ext_clos_app_right: forall R t t' u, lab_term u -> ((ext_lab_EE_ctx_red R) t t') -> ((ext_lab_EE_ctx_red R) (pterm_app u t) (pterm_app u t')).
+Proof.
+    intros.
+    destruct H0.
+    destruct H0.
+    destruct H0.
+    destruct H1.
+    exists (pterm_app u x) (pterm_app u x0).
+    split. apply star_lab_closure_app_right; auto.
+    split*. constructor 3; auto.
+    apply star_lab_closure_app_right; auto.
+
+Qed.
+
+Lemma EE_ext_clos_abs: forall R x x0 L, (forall y : VarSet.elt, y \notin L -> (ext_lab_EE_ctx_red R) (x0 ^ y) (x ^ y)) -> (ext_lab_EE_ctx_red R) (pterm_abs x0) (pterm_abs x).
 Proof.
     Admitted.
+
+Lemma EE_ext_clos_outer_sub: forall R t t' u L, (forall y : VarSet.elt, y \notin L -> (ext_lab_EE_ctx_red R) (t ^ y) (t' ^ y)) -> (ext_lab_EE_ctx_red R) (t[u]) (t'[u]).
+Proof.
+    Admitted.
+
+Lemma EE_ext_clos_inner_sub: forall R t u u', (ext_lab_EE_ctx_red R) (u) (u') -> (ext_lab_EE_ctx_red R) (t[u]) (t[u']).
+Proof.
+    Admitted.
+
+Lemma EE_ext_clos_outer_lsub: forall R t t' u L, (forall y : VarSet.elt, y \notin L -> (ext_lab_EE_ctx_red R) (t ^ y) (t' ^ y)) -> (ext_lab_EE_ctx_red R) (t[[u]]) (t'[[u]]).
+Proof.
+    Admitted.
+
+Lemma EE_ext_clos_inner_lsub: forall R t u u', (ext_lab_EE_ctx_red R) (u) (u') -> (ext_lab_EE_ctx_red R) (t[[u]]) (t[[u']]).
+Proof.
+    Admitted.
+
+(* ------------------- *)
+
+
+(*Lemma pterm_abs_EE_inversion: forall t v, (pterm_abs t) =EE v -> exists t', v = (pterm_abs t') /\ (t =EE t').*)
+(*Proof.*)
+    (*Admitted.*)
 
 Lemma red_rename_lab_xi_eq: red_rename lab_x_i_eq.
 Proof.
@@ -208,6 +241,9 @@ Lemma red_rename_lab_xe_eq: red_rename lab_x_e_eq.
 Proof.
     Admitted.
 
+Lemma red_rename_lab_lex: red_rename lab_lex.
+Proof.
+    Admitted.
 (*Lemma lx_i_open_abs: forall x x0 L, (forall y : VarSet.elt, y \notin L -> x0 ^ y-->[lx_i]x ^ y) -> pterm_abs x0-->[lx_i]pterm_abs x.*)
 (*Proof.*)
     (*Admitted.*)
@@ -216,9 +252,9 @@ Proof.
 (*Proof.*)
     (*Admitted.*)
 
-Lemma term_EE_open: forall t t' x, t =EE t' -> (t ^ x) =EE (t' ^ x).
-Proof.
-    Admitted.
+(*Lemma term_EE_open: forall t t' x, t =EE t' -> (t ^ x) =EE (t' ^ x).*)
+(*Proof.*)
+    (*Admitted.*)
 
 Lemma EE_lab_term : forall t t', lab_term t -> t =EE t' -> lab_term t'.
 Proof.
@@ -229,9 +265,9 @@ Proof.
     Admitted.
 
 
-Lemma pterm_sub_EE_inversion: forall t u v, (t[u]) =EE v -> (exists t', v = (t'[u])) \/ (exists t' u', v = (t'[u'])) \/ (exists t' u', v = (t'[[u']])).
-Proof.
-    Admitted.
+(*Lemma pterm_sub_EE_inversion: forall t u v, (t[u]) =EE v -> (exists t', v = (t'[u])) \/ (exists t' u', v = (t'[u'])) \/ (exists t' u', v = (t'[[u']])).*)
+(*Proof.*)
+    (*Admitted.*)
 
 
 Lemma EE_presv_ie: forall t t' u u', t =EE u -> u' =EE t' -> ((u -->[lx_i] u' \/ u -->[lx_e] u') -> (t -->[lx_i] t' \/ t -->[lx_e] t')).
@@ -242,7 +278,6 @@ Proof.
     left.  
     exists x x0.
     split*.
-    (*apply star_ctx_eqcc_sym in H.*)
     apply star_closure_composition with u; auto.
     split*.
     apply star_closure_composition with u'; auto.
@@ -258,6 +293,10 @@ Proof.
     apply star_closure_composition with u'; auto.
 Qed.
 
+Lemma EE_presv_lab_lex: forall t t' u u', t =EE u -> u' =EE t' -> ((u -->[lex] u') -> (t -->[lex] t')).
+Proof.
+    Admitted.
+
 Lemma lab_ex_eq_i_e: forall t t', lab_term t -> (t -->[lex] t' <-> (t -->[lx_i] t' \/ t -->[lx_e] t')).
 Proof.
     split.
@@ -267,6 +306,7 @@ Proof.
     generalize dependent t'.
     induction H1; intros.
 
+    (* -----------------------   ex -> i_e *)
     (* Base *)
     apply lab_sys_x_i_e with t s; auto. apply star_ctx_eqcc_lab_term with t0; auto*.
 
@@ -275,16 +315,16 @@ Proof.
     assert  (t-->[lx_i]t' \/ t-->[lx_e]t').
     apply IHlab_contextual_closure; auto. constructor 1; auto. admit. constructor 1; auto.
     destruct H4. 
-    left. apply EE_clos_app_left. admit. auto.
-    right. apply EE_clos_app_left. admit. auto.
+    left. apply EE_ext_clos_app_left. admit. auto.
+    right. apply EE_ext_clos_app_left. admit. auto.
 
     (* app_right *)
     apply EE_presv_ie with (u := (pterm_app t u)) (u' := (pterm_app t u')); auto.
     assert  (u-->[lx_i]u' \/ u-->[lx_e]u').
     apply IHlab_contextual_closure; auto. constructor 1; auto. admit. constructor 1; auto.
     destruct H4. 
-    left. apply EE_clos_app_right. admit. auto.
-    right. apply EE_clos_app_right. admit. auto.
+    left. apply EE_ext_clos_app_right. admit. auto.
+    right. apply EE_ext_clos_app_right. admit. auto.
 
     (* abs *)
     apply EE_presv_ie with (u := pterm_abs t) (u' := pterm_abs t'); auto.
@@ -296,9 +336,9 @@ Proof.
     apply notin_union in H5; destruct H5.
     apply notin_union in H5; destruct H5.
     destruct H4.
-    left. apply EE_clos_abs with L.
+    left. apply EE_ext_clos_abs with L.
     intros. pose proof red_rename_lab_xi_eq. apply H11 with z; auto.
-    right. apply EE_clos_abs with L.
+    right. apply EE_ext_clos_abs with L.
     intros. pose proof red_rename_lab_xe_eq. apply H11 with z; auto.
 
     (* outer sub *)
@@ -312,9 +352,9 @@ Proof.
     apply notin_union in H6; destruct H6.
     apply notin_union in H6; destruct H6.
     destruct H5.
-    left. apply EE_clos_outer_sub with L.
+    left. apply EE_ext_clos_outer_sub with L.
     intros. pose proof red_rename_lab_xi_eq. apply H13 with z; auto.
-    right. apply EE_clos_outer_sub with L.
+    right. apply EE_ext_clos_outer_sub with L.
     intros. pose proof red_rename_lab_xe_eq. apply H13 with z; auto.
 
     (* inner sub *)
@@ -324,8 +364,8 @@ Proof.
     apply EE_lab_term in H3. inversion H3; subst.
     pose proof (IHlab_contextual_closure u' H4 u H9 H5).
     destruct H6. 
-    left. apply EE_clos_inner_sub; auto.
-    right. apply EE_clos_inner_sub; auto.
+    left. apply EE_ext_clos_inner_sub; auto.
+    right. apply EE_ext_clos_inner_sub; auto.
     auto.
 
     (* outer lsub *)
@@ -339,9 +379,9 @@ Proof.
     apply notin_union in H6; destruct H6.
     apply notin_union in H6; destruct H6.
     destruct H5.
-    left. apply EE_clos_outer_lsub with L.
+    left. apply EE_ext_clos_outer_lsub with L.
     intros. pose proof red_rename_lab_xi_eq. apply H13 with z; auto.
-    right. apply EE_clos_outer_lsub with L.
+    right. apply EE_ext_clos_outer_lsub with L.
     intros. pose proof red_rename_lab_xe_eq. apply H13 with z; auto.
 
     (* inner lsub *)
@@ -356,10 +396,10 @@ Proof.
     auto.
 
 
-    (* i_e -> ex *)
+    (* -----------------------   i_e -> ex *)
     intros. destruct H0; destruct H0; destruct H0; destruct H0; destruct H1; generalize dependent t; generalize dependent t'; induction H1; intros.
 
-    (*[> Interna <]*)
+    (*[> ------------------  Interna <]*)
     (*[> Base <]*)
     inversion H; subst. 
     exists (t1 [[t2]]) (t1 [[t2']]). 
@@ -367,179 +407,127 @@ Proof.
     constructor 8. admit. inversion H4; subst.
     constructor 1; auto.  constructor 2; subst. auto. 
     exists t s. split*. constructor 1; auto. constructor 1. constructor 3; auto.
+
+    (* app_left *)
+    apply EE_presv_lab_lex with (u := (pterm_app t u)) (u' := (pterm_app t' u)); auto.
+    apply EE_clos_app_left. admit. 
+    apply IHext_lab_contextual_closure; auto. constructor 1; auto. admit. constructor 1; auto.
+
+    (* app_right *)
+    apply EE_presv_lab_lex with (u := (pterm_app t u)) (u' := (pterm_app t u')); auto.
+    apply EE_clos_app_right. admit. 
+    apply IHext_lab_contextual_closure; auto. constructor 1; auto. admit. constructor 1; auto.
+
+    (* abs *)
+    apply EE_presv_lab_lex with (u := pterm_abs t) (u' := pterm_abs t'); auto.
+    pick_fresh z.
+    assert  (t^z-->[lex]t'^z).
+    apply H0 with z; auto. constructor 1; auto. admit. constructor 1; auto. 
+    apply notin_union in Fr; destruct Fr.
+    apply notin_union in H5; destruct H5.
+    apply notin_union in H5; destruct H5.
+    apply notin_union in H5; destruct H5.
+    apply EE_clos_abs with L.
+    intros. pose proof red_rename_lab_lex. apply H11 with z; auto.
+
+    (* outer sub *)
+    apply EE_presv_lab_lex with (u := t[u]) (u' := t'[u]); auto.
+    pick_fresh z.
+    assert  (t^z-->[lex]t'^z).
+    apply H1 with z; auto. constructor 1; auto. admit. constructor 1; auto. 
+    apply notin_union in Fr; destruct Fr.
+    apply notin_union in H6; destruct H6.
+    apply notin_union in H6; destruct H6.
+    apply notin_union in H6; destruct H6.
+    apply notin_union in H6; destruct H6.
+    apply EE_clos_outer_sub with L.
+    intros. pose proof red_rename_lab_lex. apply H13 with z; auto.
+
+    (* inner sub *)
+    apply EE_presv_lab_lex with (u := t[u]) (u' := t[u']); auto.
+    assert (u' =EE u'). constructor 1; auto.
+    assert (u =EE u). constructor 1; auto.
+    apply EE_lab_term in H3. inversion H3; subst.
+    pose proof (IHext_lab_contextual_closure u' H4 u H9 H5).
+    apply EE_clos_inner_sub; auto.
+    auto.
+
+
+    (* outer lsub *)
+    apply EE_presv_lab_lex with (u := t[[u]]) (u' := t'[[u]]); auto.
+    pick_fresh z.
+    assert  (t^z-->[lex]t'^z).
+    apply H2 with z; auto. constructor 1; auto. admit. constructor 1; auto. 
+    apply notin_union in Fr; destruct Fr.
+    apply notin_union in H7; destruct H7.
+    apply notin_union in H7; destruct H7.
+    apply notin_union in H7; destruct H7.
+    apply notin_union in H7; destruct H7.
+    apply EE_clos_outer_lsub with L.
+    intros. pose proof red_rename_lab_lex. apply H14 with z; auto.
+
+    (*[> ------------------  Externa <]*)
+    (*[> Base <]*)
+    inversion H; subst. 
+    exists (t) (s).  split*. split*.  constructor 1.  constructor 1; auto.  
+    exists (t) (s).  split*. split*.  constructor 1.  constructor 2; auto.  
+
+    (* app_left *)
+    apply EE_presv_lab_lex with (u := (pterm_app t u)) (u' := (pterm_app t' u)); auto.
+    apply EE_clos_app_left. admit. 
+    apply IHext_lab_contextual_closure; auto. constructor 1; auto. admit. constructor 1; auto.
+
+    (* app_right *)
+    apply EE_presv_lab_lex with (u := (pterm_app t u)) (u' := (pterm_app t u')); auto.
+    apply EE_clos_app_right. admit. 
+    apply IHext_lab_contextual_closure; auto. constructor 1; auto. admit. constructor 1; auto.
+
+    (* abs *)
+    apply EE_presv_lab_lex with (u := pterm_abs t) (u' := pterm_abs t'); auto.
+    pick_fresh z.
+    assert  (t^z-->[lex]t'^z).
+    apply H0 with z; auto. constructor 1; auto. admit. constructor 1; auto. 
+    apply notin_union in Fr; destruct Fr.
+    apply notin_union in H5; destruct H5.
+    apply notin_union in H5; destruct H5.
+    apply notin_union in H5; destruct H5.
+    apply EE_clos_abs with L.
+    intros. pose proof red_rename_lab_lex. apply H11 with z; auto.
+
+    (* outer sub *)
+    apply EE_presv_lab_lex with (u := t[u]) (u' := t'[u]); auto.
+    pick_fresh z.
+    assert  (t^z-->[lex]t'^z).
+    apply H1 with z; auto. constructor 1; auto. admit. constructor 1; auto. 
+    apply notin_union in Fr; destruct Fr.
+    apply notin_union in H6; destruct H6.
+    apply notin_union in H6; destruct H6.
+    apply notin_union in H6; destruct H6.
+    apply notin_union in H6; destruct H6.
+    apply EE_clos_outer_sub with L.
+    intros. pose proof red_rename_lab_lex. apply H13 with z; auto.
+
+    (* inner sub *)
+    apply EE_presv_lab_lex with (u := t[u]) (u' := t[u']); auto.
+    assert (u' =EE u'). constructor 1; auto.
+    assert (u =EE u). constructor 1; auto.
+    apply EE_lab_term in H3. inversion H3; subst.
+    pose proof (IHext_lab_contextual_closure u' H4 u H9 H5).
+    apply EE_clos_inner_sub; auto.
+    auto.
+
+
+    (* outer lsub *)
+    apply EE_presv_lab_lex with (u := t[[u]]) (u' := t'[[u]]); auto.
+    pick_fresh z.
+    assert  (t^z-->[lex]t'^z).
+    apply H2 with z; auto. constructor 1; auto. admit. constructor 1; auto. 
+    apply notin_union in Fr; destruct Fr.
+    apply notin_union in H7; destruct H7.
+    apply notin_union in H7; destruct H7.
+    apply notin_union in H7; destruct H7.
+    apply notin_union in H7; destruct H7.
+    apply EE_clos_outer_lsub with L.
+    intros. pose proof red_rename_lab_lex. apply H14 with z; auto.
 Qed.
 
-(*Lemma lab_ex_eq_i_e: forall t t', lab_term t -> (t -->[lex] t' <-> (t -->[lx_i] t' \/ t -->[lx_e] t')).*)
-(*Proof.*)
-    (*split.*)
-    (*intro.*)
-    (*destruct H0.  destruct H0. destruct H0.  destruct H1.*)
-    (*generalize dependent t.*)
-    (*generalize dependent t'.*)
-    (*induction H1; intros.*)
-
-    (*[> Base <]*)
-    (*apply lab_sys_x_i_e with t s; auto. apply star_ctx_eqcc_lab_term with t0; auto*.*)
-
-    (*[> app left <]*)
-    (*assert (H4 := pterm_app_EE_inversion H2).*)
-    (*apply star_ctx_eqcc_sym in H3.*)
-    (*assert (H5 := pterm_app_EE_inversion H3).*)
-    (*destruct H4.  destruct H4.  destruct H4.  destruct H6.  *)
-    (*destruct H5.  destruct H5.  destruct H5.  destruct H8.*)
-    (*subst. inversion H0; subst.  apply star_ctx_eqcc_sym in H8.*)
-    (*assert (x1-->[lx_i]x \/ x1-->[lx_e]x).  apply IHlab_contextual_closure; auto.*)
-    (*destruct H4. left. *)
-    (*destruct H4. destruct H4. destruct H4. destruct H5.*)
-    (*exists (pterm_app x3 u) (pterm_app x4 u).*)
-    (*split. apply star_closure_composition with (pterm_app x1 u).*)
-    (*apply star_lab_closure_app_right. auto. apply star_ctx_eqcc_sym in H9. auto.*)
-    (*apply star_lab_closure_app_left. auto. auto.*)
-    (*split. constructor 2; auto. apply star_closure_composition with (pterm_app x u).*)
-    (*apply star_lab_closure_app_left; auto. apply star_lab_closure_app_right; auto.*)
-    (*admit.*)
-    (*right.*)
-    (*destruct H4. destruct H4. destruct H4. destruct H5.*)
-    (*exists (pterm_app x3 u) (pterm_app x4 u).*)
-    (*split. apply star_closure_composition with (pterm_app x1 u).*)
-    (*apply star_lab_closure_app_right. auto. apply star_ctx_eqcc_sym in H9. auto.*)
-    (*apply star_lab_closure_app_left. auto. auto.*)
-    (*split. constructor 2; auto. apply star_closure_composition with (pterm_app x u).*)
-    (*apply star_lab_closure_app_left; auto. apply star_lab_closure_app_right; auto.*)
-    (*admit.*)
-
-    (*[> app right <]*)
-    (*assert (H4 := pterm_app_EE_inversion H2).*)
-    (*apply star_ctx_eqcc_sym in H3.*)
-    (*assert (H5 := pterm_app_EE_inversion H3).*)
-    (*destruct H4.  destruct H4.  destruct H4.  destruct H6.  *)
-    (*destruct H5.  destruct H5.  destruct H5.  destruct H8.*)
-    (*subst. inversion H0; subst.  apply star_ctx_eqcc_sym in H9.*)
-    (*assert (x2-->[lx_i]x0 \/ x2-->[lx_e]x0).  apply IHlab_contextual_closure; auto.*)
-    (*destruct H4. left. *)
-    (*destruct H4. destruct H4. destruct H4. destruct H5.*)
-    (*exists (pterm_app t x3) (pterm_app t x4).*)
-    (*split. apply star_closure_composition with (pterm_app x1 x3).*)
-    (*apply star_lab_closure_app_right. auto.  auto.*)
-    (*apply star_lab_closure_app_left. admit. apply star_ctx_eqcc_sym in H8. auto. *)
-    (*split. constructor 3; auto. apply star_closure_composition with (pterm_app x x4).*)
-    (*apply star_lab_closure_app_left; auto. admit. apply star_lab_closure_app_right; auto.*)
-    (*admit.*)
-    (*right.*)
-    (*destruct H4. destruct H4. destruct H4. destruct H5.*)
-    (*exists (pterm_app t x3) (pterm_app t x4).*)
-    (*split. apply star_closure_composition with (pterm_app x1 x3).*)
-    (*apply star_lab_closure_app_right. auto.  auto.*)
-    (*apply star_lab_closure_app_left. admit. apply star_ctx_eqcc_sym in H8. auto. *)
-    (*split. constructor 3; auto. apply star_closure_composition with (pterm_app x x4).*)
-    (*apply star_lab_closure_app_left; auto. admit. apply star_lab_closure_app_right; auto.*)
-    (*admit.*)
-
-    (*[> abs <]*)
-    (*assert (H4 := pterm_abs_EE_inversion H2).*)
-    (*apply star_ctx_eqcc_sym in H3.*)
-    (*assert (H5 := pterm_abs_EE_inversion H3).*)
-    (*destruct H4.  destruct H4. *)
-    (*destruct H5.  destruct H5. *)
-    (*subst. inversion H1; subst. *)
-
-    (*assert ((forall y, y \notin (L \u L0) -> x0 ^ y -->[lx_i] x ^ y) \/  (forall y, y \notin (L \u L0) -> x0 ^ y -->[lx_e] x ^ y )).*)
-    (*pick_fresh z.*)
-    (*apply term_EE_open with t' x z in H6.*)
-    (*apply term_EE_open with t x0 z in H7.*)
-    (*apply notin_union in Fr. destruct Fr.  apply notin_union in H4. destruct H4.  *)
-    (*apply notin_union in H4. destruct H4.  apply notin_union in H4. destruct H4.  *)
-    (*apply notin_union in H4. destruct H4.  *)
-    (*pose proof (H5 z H12); auto.*)
-    (*apply star_ctx_eqcc_sym in H7.*)
-    (*pose proof (H0 z H4 (x ^ z) H6 (x0 ^ z) H13 H7). *)
-    (*clear H11 H10. auto.*)
-    (*destruct H14.*)
-    (*left. intros.*)
-    (*pose proof red_rename_lab_xi_eq.*)
-    (*apply H14 with z; auto.*)
-    (*right; intros.*)
-    (*pose proof red_rename_lab_xe_eq.*)
-    (*apply H14 with z; auto.*)
-    (*destruct H4. *)
-    (*left. apply lx_i_open_abs with (L \u L0); auto.*)
-    (*right. apply lx_e_open_abs with (L \u L0); auto.*)
-
-    (*[> sub <]*)
-
-    (*pose proof H2. apply pterm_sub_EE_inversion in H2. *)
-    (*pose proof H4. apply star_ctx_eqcc_sym in H4. apply pterm_sub_EE_inversion in H4. *)
-    (*destruct H2. destruct H2; subst. *)
-    (*destruct H4. destruct H2; subst.*)
-    (*admit.*)
-    (*destruct H2. destruct H2; subst. destruct H2; subst.*)
-
-
-    (*[>fail.<]*)
-    (*Focus 6. [> u --> u' <]*)
-    (*[>inversion H2; subst.<]*)
-    (*[>inversion H3; subst.<]*)
-    (*left. exists (t [[u]]) (t [[u']]). split. auto.*)
-    (*split*. *)
-    (*apply EE_lab_term in H3.*)
-    (*inversion H3; subst.*)
-    (*apply lab_sys_lx_term_is_sys_Bx in H0; auto.*)
-    (*inversion H0; subst.*)
-    (*constructor 1.  constructor 1. auto. auto.*)
-    (*constructor 1.  constructor 1. auto. constructor 2; auto. *)
-    (*auto.*)
-    (*[>constructor 6. constructor 2. auto. admit. constructor 2; auto. <]*)
-    (*[>constructor 1; auto. constructor 2; auto. admit. [> !!! <]<]*)
-    (*[>inversion H2; subst. inversion H4; subst. inversion H4; subst.<]*)
-    (*[>inversion H2; subst. inversion H4; subst. inversion H4; subst.<]*)
-    (*[>inversion H2; subst. inversion H4; subst. inversion H4; subst.<]*)
-    (*[>inversion H2; subst. inversion H5; subst.<]*)
-
-    (*Focus 4.*)
-    (*[> i_e -> ex <]*)
-    (*intros. destruct H0; destruct H0; destruct H0; destruct H0; destruct H1; generalize dependent t; generalize dependent t'; induction H1; intros.*)
-
-    (*[> Interna <]*)
-    (*[> Base <]*)
-    (*inversion H; subst. *)
-    (*exists (t1 [[t2]]) (t1 [[t2']]). *)
-    (*split*. split*. *)
-    (*constructor 8. admit. inversion H4; subst.*)
-    (*constructor 1; auto.  constructor 2; subst. auto. *)
-    (*exists t s. split*. constructor 1; auto. constructor 1. constructor 3; auto.*)
-
-    (*[> app_l <]*)
-    (*assert (H4 := pterm_app_EE_inversion H2).*)
-    (*apply star_ctx_eqcc_sym in H3.*)
-    (*assert (H5 := pterm_app_EE_inversion H3).*)
-    (*destruct H4.  destruct H4.  destruct H4.  destruct H6.  *)
-    (*destruct H5.  destruct H5.  destruct H5.  destruct H8.*)
-    (*subst. inversion H0; subst.  apply star_ctx_eqcc_sym in H8.*)
-    (*assert ( x1-->[lex]x ). apply IHext_lab_contextual_closure; auto. *)
-    (*destruct H4.  destruct H4.  destruct H4.  destruct H5.*)
-    (*exists (pterm_app x3 u) (pterm_app x4 u). split*. *)
-    (*apply star_closure_composition with (pterm_app x1 u).*)
-    (*apply star_lab_closure_app_right; auto. apply star_ctx_eqcc_sym; auto.*)
-    (*apply star_lab_closure_app_left; auto. split*. constructor 2; auto.*)
-    (*apply star_closure_composition with (pterm_app x u). *)
-    (*apply star_lab_closure_app_left; auto. apply star_lab_closure_app_right; auto.*)
-    (*admit.*)
-
-    (*[> app_r <]*)
-    (*assert (H4 := pterm_app_EE_inversion H2).*)
-    (*apply star_ctx_eqcc_sym in H3.*)
-    (*assert (H5 := pterm_app_EE_inversion H3).*)
-    (*destruct H4.  destruct H4.  destruct H4.  destruct H6.  *)
-    (*destruct H5.  destruct H5.  destruct H5.  destruct H8.*)
-    (*subst. inversion H0; subst.  apply star_ctx_eqcc_sym in H9.*)
-    (*assert ( x2-->[lex]x0 ). apply IHext_lab_contextual_closure; auto. *)
-    (*destruct H4.  destruct H4.  destruct H4.  destruct H5.*)
-    (*exists (pterm_app t x3) (pterm_app t x4). split*. *)
-    (*apply star_closure_composition with (pterm_app t x2).*)
-    (*apply star_lab_closure_app_left; auto. apply star_ctx_eqcc_sym; auto.*)
-    (*apply star_lab_closure_app_right; auto. split*. constructor 3; auto.*)
-    (*apply star_closure_composition with (pterm_app x x4). *)
-    (*apply star_lab_closure_app_left; auto. admit. apply star_lab_closure_app_right; auto.*)
-    (*admit.*)
-
-(*Qed.*)
